James C - down to two debranching errors again

BranchingAssembly/Debranching.thy
@@ -35,19 +35,20 @@ definition debranch :: "b_assembly_program \<Rightarrow> assembly_program" where
   "debranch \<Pi> = finite_map_fold (block_convert (dom \<Pi>)) empty \<Pi>"
 
 function remove_continuations :: "assembly list \<Rightarrow> code_label \<Rightarrow> assembly_program \<Rightarrow> 
-    (assembly list \<times> code_label) set" where
-  "\<not> finite (dom \<Pi>) \<Longrightarrow> remove_continuations \<pi> s \<Pi> = {(\<pi>, s)}"
+    (assembly list \<times> code_label)" where
+  "\<not> finite (dom \<Pi>) \<Longrightarrow> remove_continuations \<pi> s \<Pi> = (\<pi>, s)"
 | "finite (dom \<Pi>) \<Longrightarrow> remove_continuations \<pi> s \<Pi> = (case \<Pi> s of 
-        Some (\<pi>', s') \<Rightarrow> insert (\<pi>, s) (remove_continuations (\<pi> @ \<pi>') s' (\<Pi>(s := None)))
-      | None \<Rightarrow> {(\<pi>, s)})"
+        Some (\<pi>', s') \<Rightarrow> remove_continuations (\<pi> @ \<pi>') s' (\<Pi>(s := None))
+      | None \<Rightarrow> (\<pi>, s))"
   by atomize_elim auto
 termination
   by (relation "measure (card o dom o snd o snd)") (auto, meson card_Diff1_less domI)
 
-fun state_convert :: "code_label set \<Rightarrow> b_assembly_state \<Rightarrow> assembly_state set" where
+fun state_convert :: "code_label set \<Rightarrow> b_assembly_state \<Rightarrow> assembly_state" where
   "state_convert ss (\<mu>, a, d, \<pi>, s, \<omega>) = (
     let (\<pi>', s', \<Pi>') = branch_instr_convert ss \<pi> s
-    in {(\<mu>, a, d, \<pi>'', s'', \<omega>) | \<pi>'' s''. (\<pi>'', s'') \<in> remove_continuations \<pi>' s' \<Pi>'})"
+    in let (\<pi>'', s'') = remove_continuations \<pi>' s' \<Pi>'
+    in (\<mu>, a, d, \<pi>'', s'', \<omega>))"
 
 (* conversion correctness *)
 
@@ -102,11 +103,8 @@ lemma [simp]: "finite ss \<Longrightarrow> ss \<supseteq> dom \<Pi> \<Longrighta
 lemma [simp]: "finite (dom \<Pi>) \<Longrightarrow> finite (dom (debranch \<Pi>))"
   by (simp add: debranch_def)
 
-lemma [simp]: "(\<pi>, s) \<in> remove_continuations \<pi> s \<Pi>"
-  by (induction \<pi> s \<Pi> rule: remove_continuations.induct) (simp_all split: option.splits)
-
-lemma remove_cont_extends: "(\<pi>', s') \<in> remove_continuations (\<iota> # \<pi>) s \<Pi> \<Longrightarrow> 
-    \<exists>\<pi>''. \<pi>' = \<iota> # \<pi> @ \<pi>'' \<and> (\<pi> @ \<pi>'', s') \<in> remove_continuations \<pi> s \<Pi>"
+lemma [simp]: "(\<pi>', s') = remove_continuations \<pi> s \<Pi> \<Longrightarrow>
+    (\<iota> # \<pi>', s') = remove_continuations (\<iota> # \<pi>) s \<Pi>"
   proof (induction \<pi> s \<Pi> rule: remove_continuations.induct)
   case 1
     thus ?case by simp
@@ -120,118 +118,182 @@ lemma remove_cont_extends: "(\<pi>', s') \<in> remove_continuations (\<iota> # \
       qed
   qed
 
-lemma [simp]: "\<Sigma>\<^sub>A \<in> state_convert ss \<Sigma>\<^sub>B \<Longrightarrow> assembly_output \<Sigma>\<^sub>A = b_assembly_output \<Sigma>\<^sub>B"
-  by (induction \<Sigma>\<^sub>B rule: b_assembly_output.induct, induction \<Sigma>\<^sub>A rule: assembly_output.induct) 
-     (simp split: prod.splits)
-
-lemma debranch_step: "eval_b_assembly \<Pi> \<Sigma>\<^sub>B = Some \<Sigma>\<^sub>B' \<Longrightarrow> \<Sigma>\<^sub>A \<in> state_convert (dom \<Pi>) \<Sigma>\<^sub>B \<Longrightarrow> 
-    \<exists>\<Sigma>\<^sub>A'. \<Sigma>\<^sub>A' \<in> state_convert (dom \<Pi>) \<Sigma>\<^sub>B' \<and> eval_assembly (debranch \<Pi>) \<Sigma>\<^sub>A = Some \<Sigma>\<^sub>A'"
-  proof (induction \<Pi> \<Sigma>\<^sub>B rule: eval_b_assembly.induct)
-  case (1 \<Pi> \<mu> a d s \<omega>)
+lemma [simp]: "(\<pi>', s') = remove_continuations \<pi> s \<Pi> \<Longrightarrow>
+    (\<pi>\<^sub>2 @ \<pi>', s') = remove_continuations (\<pi>\<^sub>2 @ \<pi>) s \<Pi>"
+  proof (induction \<pi> s \<Pi> rule: remove_continuations.induct)
+  case 1
+    thus ?case by simp
+  next case (2 \<Pi> \<pi> s)
     thus ?case
       proof (cases "\<Pi> s")
       case (Some ps)
-        thus ?thesis
-          proof (cases ps)
-          case (Pair \<pi>\<^sub>B s')
-            thus ?thesis
-              proof (cases "branch_instr_convert (dom \<Pi>) \<pi>\<^sub>B s'")
-              case (fields \<pi>\<^sub>A s'' \<Pi>')
-
-            
-                have X: "\<Sigma>\<^sub>A' \<in> state_convert (dom \<Pi>) (\<mu>, None, d, \<pi>\<^sub>B, s', \<omega>)" by simp
-    
-    
-                have "(case debranch \<Pi> s of 
-      Some (\<pi>', s') \<Rightarrow> Some (\<mu>, None, d, \<pi>', s', \<omega>)
-    | None \<Rightarrow> None) = Some \<Sigma>\<^sub>A'" by simp
-                with X 1 Some Pair fields show ?thesis by auto
-              qed
-          qed
+        with 2 show ?thesis by (cases ps) fastforce
       next case None
-        with 1 show ?thesis by simp
+        with 2 show ?thesis by simp
       qed
+  qed
+
+lemma [simp]: "assembly_output (state_convert ss \<Sigma>\<^sub>B) = b_assembly_output \<Sigma>\<^sub>B"
+  by (induction \<Sigma>\<^sub>B rule: b_assembly_output.induct) (simp split: prod.splits)
+
+lemma debranch_step: "eval_b_assembly \<Pi> \<Sigma>\<^sub>B = Some \<Sigma>\<^sub>B' \<Longrightarrow> 
+    eval_assembly (debranch \<Pi>) (state_convert (dom \<Pi>) \<Sigma>\<^sub>B) = Some (state_convert (dom \<Pi>) \<Sigma>\<^sub>B')"
+  proof (induction \<Pi> \<Sigma>\<^sub>B rule: eval_b_assembly.induct)
+  case (1 \<Pi> \<mu> a d s \<omega>)
+    then obtain ps where "\<Pi> s = Some ps" by (cases "\<Pi> s") simp_all
+    then obtain \<pi>\<^sub>B s' where PS: "\<Pi> s = Some (\<pi>\<^sub>B, s')" by (cases ps) simp
+    obtain \<pi>\<^sub>A s'' \<Pi>' where B: "(\<pi>\<^sub>A, s'', \<Pi>') = branch_instr_convert (dom \<Pi>) \<pi>\<^sub>B s'" 
+      by (cases "branch_instr_convert (dom \<Pi>) \<pi>\<^sub>B s'") simp
+    obtain \<pi>\<^sub>A' s''' where C: "(\<pi>\<^sub>A', s''') = remove_continuations \<pi>\<^sub>A s'' \<Pi>'"
+      by (cases "remove_continuations \<pi>\<^sub>A s'' \<Pi>'") simp
+    have S: "state_convert (dom \<Pi>) (\<mu>, None, d, \<pi>\<^sub>B, s', \<omega>) = (\<mu>, None, d, \<pi>\<^sub>A', s''', \<omega>)"
+      proof -
+        from B have "state_convert (dom \<Pi>) (\<mu>, None, d, \<pi>\<^sub>B, s', \<omega>) = (
+          let (\<pi>\<^sub>A, s'', \<Pi>') = (\<pi>\<^sub>A, s'', \<Pi>')
+          in let (\<pi>'', s'') = remove_continuations \<pi>\<^sub>A s'' \<Pi>'
+          in (\<mu>, None, d, \<pi>'', s'', \<omega>))" by simp
+        with C have "state_convert (dom \<Pi>) (\<mu>, None, d, \<pi>\<^sub>B, s', \<omega>) = (
+          let (\<pi>\<^sub>A', s''') = (\<pi>\<^sub>A', s''')
+          in (\<mu>, None, d, \<pi>\<^sub>A', s''', \<omega>))" by simp
+        thus ?thesis by simp
+      qed
+
+
+    have "debranch \<Pi> s = Some (\<pi>\<^sub>A', s''')" by simp
+    with 1 PS S show ?case by simp
   next case (2 \<Pi> \<mu> a d x \<pi>\<^sub>B s \<omega>)
-    with remove_cont_extends show ?case by (cases "branch_instr_convert (dom \<Pi>) \<pi>\<^sub>B s") fastforce
-  next case (3 \<Pi> \<mu> a d dst cmp \<pi>\<^sub>B s \<omega>)
-    thus ?case
-      proof (cases "branch_instr_convert (dom \<Pi>) \<pi>\<^sub>B s")
-      case (fields \<pi>\<^sub>A s' \<Pi>')
-        let ?n = "compute cmp (\<mu> a) a d"
-        let ?m = "if M \<in> dst then \<mu>(a := ?n) else \<mu>"
-        let ?a = "Some (if A \<in> dst then ?n else a)"
-        let ?d = "if D \<in> dst then ?n else d"
-        from 3 have SB: "\<Sigma>\<^sub>B' = (?m, ?a, ?d, \<pi>\<^sub>B, s, \<omega>)" by (simp add: Let_def)
-        from 3 fields obtain \<pi>\<^sub>A' s'' where SA: "\<Sigma>\<^sub>A = (\<mu>, Some a, d, \<pi>\<^sub>A', s'', \<omega>) \<and> 
-          (\<pi>\<^sub>A', s'') \<in> remove_continuations (CAssm dst cmp # \<pi>\<^sub>A) s' \<Pi>'" by fastforce
-        with remove_cont_extends obtain \<pi>\<^sub>A'' where P: "\<pi>\<^sub>A' = CAssm dst cmp # \<pi>\<^sub>A @ \<pi>\<^sub>A'' \<and> 
-          (\<pi>\<^sub>A @ \<pi>\<^sub>A'', s'') \<in> remove_continuations \<pi>\<^sub>A s' \<Pi>'" by fastforce
-        have "eval_assembly (debranch \<Pi>) (\<mu>, Some a, d, CAssm dst cmp # \<pi>\<^sub>A @ \<pi>\<^sub>A'', s'', \<omega>) = 
-          Some (?m, ?a, ?d, \<pi>\<^sub>A @ \<pi>\<^sub>A'', s'', \<omega>)" by (simp add: Let_def)
-        with 3 SA SB P fields show ?thesis by fastforce
+    obtain \<pi>\<^sub>A s' \<Pi>' where B: "(\<pi>\<^sub>A, s', \<Pi>') = branch_instr_convert (dom \<Pi>) \<pi>\<^sub>B s"
+      by (cases "branch_instr_convert (dom \<Pi>) \<pi>\<^sub>B s") simp
+    obtain \<pi>\<^sub>A' s'' where C: "(\<pi>\<^sub>A', s'') = remove_continuations \<pi>\<^sub>A s' \<Pi>'"
+      by (cases "remove_continuations \<pi>\<^sub>A s' \<Pi>'") simp
+    from B C have A: "state_convert (dom \<Pi>) (\<mu>, a, d, ABAssm x # \<pi>\<^sub>B, s, \<omega>) = 
+        (\<mu>, a, d, AAssm x # \<pi>\<^sub>A', s'', \<omega>)"
+      proof -
+        from B have "state_convert (dom \<Pi>) (\<mu>, a, d, ABAssm x # \<pi>\<^sub>B, s, \<omega>) = (
+          let (\<pi>', s', \<Pi>') = (
+            let (\<pi>', s', \<Pi>) = (\<pi>\<^sub>A, s', \<Pi>')
+            in (AAssm x # \<pi>', s', \<Pi>))
+          in let (\<pi>'', s'') = remove_continuations \<pi>' s' \<Pi>'
+          in (\<mu>, a, d, \<pi>'', s'', \<omega>))" by simp
+        with C have "state_convert (dom \<Pi>) (\<mu>, a, d, ABAssm x # \<pi>\<^sub>B, s, \<omega>) = (
+          let (\<pi>'', s'') = (AAssm x # \<pi>\<^sub>A', s'')
+          in (\<mu>, a, d, \<pi>'', s'', \<omega>))" by simp
+        thus ?thesis by simp
       qed
+    have "state_convert (dom \<Pi>) (\<mu>, Some x, d, \<pi>\<^sub>B, s, \<omega>) = (\<mu>, Some x, d, \<pi>\<^sub>A', s'', \<omega>)"
+      proof - 
+        from B have "state_convert (dom \<Pi>) (\<mu>, Some x, d, \<pi>\<^sub>B, s, \<omega>) = (
+          let (\<pi>\<^sub>A, s', \<Pi>') = (\<pi>\<^sub>A, s', \<Pi>')
+          in let (\<pi>\<^sub>A', s'') = remove_continuations \<pi>\<^sub>A s' \<Pi>'
+          in (\<mu>, Some x, d, \<pi>\<^sub>A', s'', \<omega>))" by simp
+        with C have "state_convert (dom \<Pi>) (\<mu>, Some x, d, \<pi>\<^sub>B, s, \<omega>) = (
+          let (\<pi>\<^sub>A', s'') = (\<pi>\<^sub>A', s'')
+          in (\<mu>, Some x, d, \<pi>\<^sub>A', s'', \<omega>))" by simp
+        thus ?thesis by simp
+      qed
+    with 2 A show ?case by simp
+  next case (3 \<Pi> \<mu> a d dst cmp \<pi>\<^sub>B s \<omega>)
+    let ?n = "compute cmp (\<mu> a) a d"
+    let ?m = "if M \<in> dst then \<mu>(a := ?n) else \<mu>"
+    let ?a = "Some (if A \<in> dst then ?n else a)"
+    let ?d = "if D \<in> dst then ?n else d"
+    obtain \<pi>\<^sub>A s' \<Pi>' where B: "(\<pi>\<^sub>A, s', \<Pi>') = branch_instr_convert (dom \<Pi>) \<pi>\<^sub>B s"
+      by (cases "branch_instr_convert (dom \<Pi>) \<pi>\<^sub>B s") simp
+    obtain \<pi>\<^sub>A' s'' where C: "(\<pi>\<^sub>A', s'') = remove_continuations \<pi>\<^sub>A s' \<Pi>'" 
+      by (cases "remove_continuations \<pi>\<^sub>A s' \<Pi>'") simp
+    have S: "state_convert (dom \<Pi>) (?m, ?a, ?d, \<pi>\<^sub>B, s, \<omega>) = (?m, ?a, ?d, \<pi>\<^sub>A', s'', \<omega>)" 
+      proof -
+        from B have "state_convert (dom \<Pi>) (?m, ?a, ?d, \<pi>\<^sub>B, s, \<omega>) = (
+          let (\<pi>\<^sub>A, s', \<Pi>') = (\<pi>\<^sub>A, s', \<Pi>')
+          in let (\<pi>'', s'') = remove_continuations \<pi>\<^sub>A s' \<Pi>'
+          in (?m, ?a, ?d, \<pi>'', s'', \<omega>))" by simp
+        with C have "state_convert (dom \<Pi>) (?m, ?a, ?d, \<pi>\<^sub>B, s, \<omega>) = (
+          let (\<pi>\<^sub>A', s'') = (\<pi>\<^sub>A', s'')
+          in (?m, ?a, ?d, \<pi>\<^sub>A', s'', \<omega>))" by simp
+        thus ?thesis by simp
+      qed
+    have "state_convert (dom \<Pi>) (\<mu>, Some a, d, CBAssm dst cmp # \<pi>\<^sub>B, s, \<omega>) = 
+        (\<mu>, Some a, d, CAssm dst cmp # \<pi>\<^sub>A', s'', \<omega>)" 
+      proof -
+        from B have "state_convert (dom \<Pi>) (\<mu>, Some a, d, CBAssm dst cmp # \<pi>\<^sub>B, s, \<omega>) = (
+          let (\<pi>\<^sub>A, s', \<Pi>') = (
+            let (\<pi>', s', \<Pi>) = (\<pi>\<^sub>A, s', \<Pi>')
+            in (CAssm dst cmp # \<pi>', s', \<Pi>))
+          in let (\<pi>'', s'') = remove_continuations \<pi>\<^sub>A s' \<Pi>'
+          in (\<mu>, Some a, d, \<pi>'', s'', \<omega>))" by simp
+        with C have "state_convert (dom \<Pi>) (\<mu>, Some a, d, CBAssm dst cmp # \<pi>\<^sub>B, s, \<omega>) = (
+          let (\<pi>\<^sub>A', s'') = (CAssm dst cmp # \<pi>\<^sub>A', s'')
+          in (\<mu>, Some a, d, \<pi>\<^sub>A', s'', \<omega>))" by simp
+        thus ?thesis by simp
+      qed
+    with 3 S show ?case by (simp add: Let_def)
   next case 4
     thus ?case by simp
-  next case (5 \<Pi> \<mu> a d jmp \<pi>\<^sub>B\<^sub>t \<pi>\<^sub>B\<^sub>f \<pi>\<^sub>B s \<omega>)
+  next case (5 \<Pi> \<mu> a d jmp \<pi>\<^sub>B\<^sub>t \<pi>\<^sub>B\<^sub>f \<pi>\<^sub>B s \<omega>)    
     let ?s\<^sub>e = "new_label (dom \<Pi>)"
-    show ?case
-      proof (cases "branch_instr_convert (dom \<Pi> \<union> {?s\<^sub>e}) \<pi>\<^sub>B\<^sub>t ?s\<^sub>e")
-      case (fields \<pi>\<^sub>t' s\<^sub>t \<Pi>\<^sub>1) note BE = fields
-        thus ?thesis
-          proof (cases "branch_instr_convert (dom \<Pi> \<union> dom \<Pi>\<^sub>1 \<union> {?s\<^sub>e}) \<pi>\<^sub>B\<^sub>f ?s\<^sub>e")
-          case (fields \<pi>\<^sub>f' s\<^sub>f \<Pi>\<^sub>2) note BF = fields
-            thus ?thesis
-              proof (cases "branch_instr_convert (dom \<Pi> \<union> dom \<Pi>\<^sub>1 \<union> dom \<Pi>\<^sub>2 \<union> {?s\<^sub>e}) \<pi>\<^sub>B s")
-              case (fields \<pi>' s' \<Pi>\<^sub>3)
-                thus ?thesis
-                  proof (cases "should_jump d jmp")
-                  case True
-                    from 5 True have SB: "\<Sigma>\<^sub>B' = (\<mu>, a, d, \<pi>\<^sub>B\<^sub>t @ \<pi>\<^sub>B, s, \<omega>)" by simp
-                    from 5 have SA: "\<Sigma>\<^sub>A \<in> state_convert (dom \<Pi>) (\<mu>, a, d, IBAssm jmp \<pi>\<^sub>B\<^sub>t \<pi>\<^sub>B\<^sub>f # \<pi>\<^sub>B, s, \<omega>)" by simp
-                
-            from BE BF fields have "state_convert (dom \<Pi>) (\<mu>, a, d, IBAssm jmp \<pi>\<^sub>B\<^sub>t \<pi>\<^sub>B\<^sub>f # \<pi>\<^sub>B, s, \<omega>) = (
-                let (\<pi>', s', \<Pi>') = (JAssm jmp s\<^sub>t # \<pi>\<^sub>f', s\<^sub>f, \<Pi>\<^sub>1 ++ \<Pi>\<^sub>2 ++ \<Pi>\<^sub>3 ++ [s\<^sub>t \<mapsto> (\<pi>\<^sub>t', s\<^sub>t), ?s\<^sub>e \<mapsto> (\<pi>', s')])
-                in {(\<mu>, a, d, \<pi>'', s'', \<omega>) | \<pi>'' s''. (\<pi>'', s'') \<in> remove_continuations (JAssm jmp s\<^sub>t # \<pi>\<^sub>f') s\<^sub>f \<Pi>'})" by (simp add: Let_def)
-            
-                
-            
-                    have X: "\<Sigma>\<^sub>A' \<in> state_convert (dom \<Pi>) (\<mu>, a, d, \<pi>\<^sub>B\<^sub>t @ \<pi>\<^sub>B, s, \<omega>)" by simp
-                
-                
-                    have "eval_assembly (debranch \<Pi>) \<Sigma>\<^sub>A = Some \<Sigma>\<^sub>A'" by simp
-                    with SB SA X show ?thesis by metis
-                  next case False
-                    from 5 False have SB: "\<Sigma>\<^sub>B' = (\<mu>, a, d, \<pi>\<^sub>B\<^sub>f @ \<pi>\<^sub>B, s, \<omega>)" by fastforce
-                    from 5 have "\<Sigma>\<^sub>A \<in> state_convert (dom \<Pi>) (\<mu>, a, d, IBAssm jmp \<pi>\<^sub>B\<^sub>t \<pi>\<^sub>B\<^sub>f # \<pi>\<^sub>B, s, \<omega>)" by simp
-                
-                
-                    have X: "\<Sigma>\<^sub>A' \<in> state_convert (dom \<Pi>) (\<mu>, a, d, \<pi>\<^sub>B\<^sub>f @ \<pi>\<^sub>B, s, \<omega>)" by simp
-                
-                
-                    have "eval_assembly (debranch \<Pi>) \<Sigma>\<^sub>A = Some \<Sigma>\<^sub>A'" by simp
-                    with SB X show ?thesis by metis
-                  qed
-              qed
-          qed
-      qed
+    obtain \<pi>\<^sub>A s' \<Pi>' where B: "(\<pi>\<^sub>A, s', \<Pi>') = branch_instr_convert (dom \<Pi>) \<pi>\<^sub>B s"
+      by (cases "branch_instr_convert (dom \<Pi>) \<pi>\<^sub>B s") simp
+
+have "branch_instr_convert (dom \<Pi>) (IBAssm jmp \<pi>\<^sub>B\<^sub>t \<pi>\<^sub>B\<^sub>f # \<pi>\<^sub>B) s = (
+    let (\<pi>\<^sub>t', s\<^sub>t, \<Pi>\<^sub>1) = branch_instr_convert (dom \<Pi> \<union> {?s\<^sub>e}) \<pi>\<^sub>B\<^sub>t ?s\<^sub>e
+    in let (\<pi>\<^sub>f', s\<^sub>f, \<Pi>\<^sub>2) = branch_instr_convert (dom \<Pi> \<union> dom \<Pi>\<^sub>1 \<union> {?s\<^sub>e}) \<pi>\<^sub>B\<^sub>f ?s\<^sub>e
+    in let (\<pi>', s', \<Pi>\<^sub>3) = branch_instr_convert (dom \<Pi> \<union> dom \<Pi>\<^sub>1 \<union> dom \<Pi>\<^sub>2 \<union> {?s\<^sub>e}) \<pi>\<^sub>B s
+    in (JAssm jmp s\<^sub>t # \<pi>\<^sub>f', s\<^sub>f, \<Pi>\<^sub>1 ++ \<Pi>\<^sub>2 ++ \<Pi>\<^sub>3 ++ [s\<^sub>t \<mapsto> (\<pi>\<^sub>t', s\<^sub>t), ?s\<^sub>e \<mapsto> (\<pi>', s')]))" by (simp add: Let_def)
+
+have "state_convert (dom \<Pi>) (\<mu>, a, d, IBAssm jmp \<pi>\<^sub>B\<^sub>t \<pi>\<^sub>B\<^sub>f # \<pi>\<^sub>B, s, \<omega>) = (
+    let (\<pi>', s', \<Pi>') = branch_instr_convert (dom \<Pi>) (IBAssm jmp \<pi>\<^sub>B\<^sub>t \<pi>\<^sub>B\<^sub>f # \<pi>\<^sub>B) s
+    in let (\<pi>'', s'') = remove_continuations \<pi>' s' \<Pi>'
+    in (\<mu>, a, d, \<pi>'', s'', \<omega>))" by simp
+    
+
+have "state_convert (dom \<Pi>) (\<mu>, a, d, (if should_jump d jmp then \<pi>\<^sub>B\<^sub>t else \<pi>\<^sub>B\<^sub>f) @ \<pi>\<^sub>B, s, \<omega>) = (
+    let (\<pi>', s', \<Pi>') = branch_instr_convert (dom \<Pi>) ((if should_jump d jmp then \<pi>\<^sub>B\<^sub>t else \<pi>\<^sub>B\<^sub>f) @ \<pi>\<^sub>B) s
+    in let (\<pi>'', s'') = remove_continuations \<pi>' s' \<Pi>'
+    in (\<mu>, a, d, \<pi>'', s'', \<omega>))" by simp
+    
+
+
+    have "eval_assembly (debranch \<Pi>) (state_convert (dom \<Pi>) (\<mu>, a, d, IBAssm jmp \<pi>\<^sub>B\<^sub>t \<pi>\<^sub>B\<^sub>f # \<pi>\<^sub>B, s, \<omega>)) = Some (state_convert (dom \<Pi>) (\<mu>, a, d, (if should_jump d jmp then \<pi>\<^sub>B\<^sub>t else \<pi>\<^sub>B\<^sub>f) @ \<pi>\<^sub>B, s, \<omega>))" by simp
+    with 5 show ?case by simp
   next case (6 \<Pi> \<mu> a d \<pi>\<^sub>B s \<omega>)
-    with remove_cont_extends show ?case by (cases "branch_instr_convert (dom \<Pi>) \<pi>\<^sub>B s") fastforce
+    obtain \<pi>\<^sub>A s' \<Pi>' where B: "(\<pi>\<^sub>A, s', \<Pi>') = branch_instr_convert (dom \<Pi>) \<pi>\<^sub>B s"
+      by (cases "branch_instr_convert (dom \<Pi>) \<pi>\<^sub>B s") simp
+    obtain \<pi>\<^sub>A' s'' where C: "(\<pi>\<^sub>A', s'') = remove_continuations \<pi>\<^sub>A s' \<Pi>'"
+      by (cases "remove_continuations \<pi>\<^sub>A s' \<Pi>'") simp
+    hence A: "state_convert (dom \<Pi>) (\<mu>, a, d, PBAssm # \<pi>\<^sub>B, s, \<omega>) = (\<mu>, a, d, PAssm # \<pi>\<^sub>A', s'', \<omega>)"
+      proof -
+        from B have "state_convert (dom \<Pi>) (\<mu>, a, d, PBAssm # \<pi>\<^sub>B, s, \<omega>) = (
+          let (\<pi>', s', \<Pi>') = (
+            let (\<pi>', s', \<Pi>) = (\<pi>\<^sub>A, s', \<Pi>')
+            in (PAssm # \<pi>', s', \<Pi>))
+          in let (\<pi>'', s'') = remove_continuations \<pi>' s' \<Pi>'
+          in (\<mu>, a, d, \<pi>'', s'', \<omega>))" by simp
+        with C have "state_convert (dom \<Pi>) (\<mu>, a, d, PBAssm # \<pi>\<^sub>B, s, \<omega>) = (
+          let (\<pi>'', s'') = (PAssm # \<pi>\<^sub>A', s'')
+          in (\<mu>, a, d, \<pi>'', s'', \<omega>))" by simp
+        thus ?thesis by simp
+      qed
+    have "state_convert (dom \<Pi>) (\<mu>, a, d, \<pi>\<^sub>B, s, d # \<omega>) = (\<mu>, a, d, \<pi>\<^sub>A', s'', d # \<omega>)" 
+      proof - 
+        from B have "state_convert (dom \<Pi>) (\<mu>, a, d, \<pi>\<^sub>B, s, d # \<omega>) = (
+          let (\<pi>\<^sub>A, s', \<Pi>') = (\<pi>\<^sub>A, s', \<Pi>')
+          in let (\<pi>\<^sub>A', s'') = remove_continuations \<pi>\<^sub>A s' \<Pi>'
+          in (\<mu>, a, d, \<pi>\<^sub>A', s'', d # \<omega>))" by simp
+        with C have "state_convert (dom \<Pi>) (\<mu>, a, d, \<pi>\<^sub>B, s, d # \<omega>) = (
+          let (\<pi>\<^sub>A', s'') = (\<pi>\<^sub>A', s'')
+          in (\<mu>, a, d, \<pi>\<^sub>A', s'', d # \<omega>))" by simp
+        thus ?thesis by simp
+      qed
+    with 6 A show ?case by simp
   qed 
 
 theorem debranching_correct [simp]: "iterate (eval_b_assembly \<Pi>) \<Sigma>\<^sub>B \<Sigma>\<^sub>B' \<Longrightarrow> 
-  \<Sigma>\<^sub>A \<in> state_convert (dom \<Pi>) \<Sigma>\<^sub>B \<Longrightarrow> 
-    \<exists>\<Sigma>\<^sub>A'. \<Sigma>\<^sub>A' \<in> state_convert (dom \<Pi>) \<Sigma>\<^sub>B' \<and> iterate (eval_assembly (debranch \<Pi>)) \<Sigma>\<^sub>A \<Sigma>\<^sub>A'"
+    iterate (eval_assembly (debranch \<Pi>)) (state_convert (dom \<Pi>) \<Sigma>\<^sub>B) (state_convert (dom \<Pi>) \<Sigma>\<^sub>B')"
   proof (induction "eval_b_assembly \<Pi>" \<Sigma>\<^sub>B \<Sigma>\<^sub>B' rule: iterate.induct)
   case iter_refl
-    thus ?case by fastforce
-  next case (iter_step \<Sigma>\<^sub>B \<Sigma>\<^sub>B' \<Sigma>\<^sub>B'')
-    then obtain \<Sigma>\<^sub>A' where S: "\<Sigma>\<^sub>A' \<in> state_convert (dom \<Pi>) \<Sigma>\<^sub>B' \<and> 
-      iterate (eval_assembly (debranch \<Pi>)) \<Sigma>\<^sub>A \<Sigma>\<^sub>A'" by blast
-    with iter_step debranch_step obtain \<Sigma>\<^sub>A'' where
-      "\<Sigma>\<^sub>A'' \<in> state_convert (dom \<Pi>) \<Sigma>\<^sub>B'' \<and> eval_assembly (debranch \<Pi>) \<Sigma>\<^sub>A' = Some \<Sigma>\<^sub>A''" by blast
-    with S have "\<Sigma>\<^sub>A'' \<in> state_convert (dom \<Pi>) \<Sigma>\<^sub>B'' \<and> iterate (eval_assembly (debranch \<Pi>)) \<Sigma>\<^sub>A \<Sigma>\<^sub>A''" 
-      by fastforce
-    thus ?case by blast
+    thus ?case by auto
+  next case iter_step
+    with debranch_step show ?case by auto
   qed
 
 end
