TotalCorrectness.thy
@@ -7,12 +7,12 @@ imports
 begin
 
 definition state_convert :: "stack_program \<Rightarrow> stack_state \<Rightarrow> machine_state set" where
-  "state_convert \<Pi> \<Sigma>\<^sub>S = { \<Sigma>\<^sub>M | \<Sigma>\<^sub>B \<Sigma>\<^sub>A \<Sigma>\<^sub>M. 
+  "state_convert \<Pi> \<Sigma>\<^sub>S = { \<Sigma>\<^sub>M | \<Sigma>\<^sub>B \<Sigma>\<^sub>M. 
     \<Sigma>\<^sub>B \<in> StackToAssembly.state_convert \<Sigma>\<^sub>S \<and> 
-      \<Sigma>\<^sub>A \<in> Debranching.state_convert (dom (StackToAssembly.program_convert \<Pi>)) \<Sigma>\<^sub>B \<and>
-        \<Sigma>\<^sub>M \<in> AssemblyToMachine.state_convert
-          (linearize (debranch (StackToAssembly.program_convert \<Pi>))) 
-            (Linearization.state_convert \<Sigma>\<^sub>A) }"
+      \<Sigma>\<^sub>M \<in> AssemblyToMachine.state_convert
+        (linearize (debranch (StackToAssembly.program_convert \<Pi>))) 
+          (Linearization.state_convert 
+            (Debranching.state_convert (dom (StackToAssembly.program_convert \<Pi>)) \<Sigma>\<^sub>B)) }"
 
 definition program_convert :: "stack_program \<Rightarrow> machine_program" where
   "program_convert \<Pi> =
@@ -23,9 +23,9 @@ theorem output_equivalence: "\<Sigma>\<^sub>M \<in> state_convert \<Pi> \<Sigma>
     let ?\<Pi>\<^sub>B = "StackToAssembly.program_convert \<Pi>"
     let ?\<Pi>\<^sub>A = "linearize (debranch ?\<Pi>\<^sub>B)"
     assume "\<Sigma>\<^sub>M \<in> state_convert \<Pi> \<Sigma>\<^sub>S"
-    with state_convert_def obtain \<Sigma>\<^sub>B \<Sigma>\<^sub>A where B: "\<Sigma>\<^sub>B \<in> StackToAssembly.state_convert \<Sigma>\<^sub>S \<and> 
-      \<Sigma>\<^sub>A \<in> Debranching.state_convert (dom ?\<Pi>\<^sub>B) \<Sigma>\<^sub>B \<and>
-        \<Sigma>\<^sub>M \<in> AssemblyToMachine.state_convert ?\<Pi>\<^sub>A (Linearization.state_convert \<Sigma>\<^sub>A)" by blast
+    with state_convert_def obtain \<Sigma>\<^sub>B where B: "\<Sigma>\<^sub>B \<in> StackToAssembly.state_convert \<Sigma>\<^sub>S \<and> 
+      \<Sigma>\<^sub>M \<in> AssemblyToMachine.state_convert ?\<Pi>\<^sub>A (Linearization.state_convert 
+        (Debranching.state_convert (dom ?\<Pi>\<^sub>B) \<Sigma>\<^sub>B))" by blast
     thus ?thesis by auto
   qed
 
@@ -42,23 +42,25 @@ theorem total_correctness: "finite (dom \<Pi>) \<Longrightarrow> iterate (eval_s
     let ?\<Pi>\<^sub>A = "debranch ?\<Pi>\<^sub>B"
     let ?\<Pi>\<^sub>M = "AssemblyToMachine.program_convert (linearize ?\<Pi>\<^sub>A)"
     assume "\<Sigma>\<^sub>M \<in> state_convert \<Pi> \<Sigma>\<^sub>S"
-    with state_convert_def obtain \<Sigma>\<^sub>B \<Sigma>\<^sub>A where B: "\<Sigma>\<^sub>B \<in> StackToAssembly.state_convert \<Sigma>\<^sub>S \<and> 
-      \<Sigma>\<^sub>A \<in> Debranching.state_convert (dom ?\<Pi>\<^sub>B) \<Sigma>\<^sub>B \<and>
-        \<Sigma>\<^sub>M \<in> AssemblyToMachine.state_convert (linearize ?\<Pi>\<^sub>A) (Linearization.state_convert \<Sigma>\<^sub>A)" 
+    with state_convert_def obtain \<Sigma>\<^sub>B where B: "\<Sigma>\<^sub>B \<in> StackToAssembly.state_convert \<Sigma>\<^sub>S \<and> 
+      \<Sigma>\<^sub>M \<in> AssemblyToMachine.state_convert (linearize ?\<Pi>\<^sub>A) 
+        (Linearization.state_convert (Debranching.state_convert (dom ?\<Pi>\<^sub>B) \<Sigma>\<^sub>B))" 
       by blast
     with ES stack_to_assembly_correct obtain \<Sigma>\<^sub>B' where SB': 
       "\<Sigma>\<^sub>B' \<in> StackToAssembly.state_convert \<Sigma>\<^sub>S' \<and> iterate (eval_b_assembly ?\<Pi>\<^sub>B) \<Sigma>\<^sub>B \<Sigma>\<^sub>B'" by blast
-    with ES DA B debranching_correct obtain \<Sigma>\<^sub>A' where SA':
-      "\<Sigma>\<^sub>A' \<in> Debranching.state_convert (dom ?\<Pi>\<^sub>B) \<Sigma>\<^sub>B' \<and> iterate (eval_assembly ?\<Pi>\<^sub>A) \<Sigma>\<^sub>A \<Sigma>\<^sub>A'" by blast
+    with ES DA B debranching_correct have SA': "iterate (eval_assembly ?\<Pi>\<^sub>A)
+      (Debranching.state_convert (dom ?\<Pi>\<^sub>B) \<Sigma>\<^sub>B) (Debranching.state_convert (dom ?\<Pi>\<^sub>B) \<Sigma>\<^sub>B')" by blast
     with DF linearization_correct have SL': "iterate (eval_l_assembly (linearize ?\<Pi>\<^sub>A)) 
-      (Linearization.state_convert \<Sigma>\<^sub>A) (Linearization.state_convert \<Sigma>\<^sub>A')" by blast
+      (Linearization.state_convert (Debranching.state_convert (dom ?\<Pi>\<^sub>B) \<Sigma>\<^sub>B)) 
+        (Linearization.state_convert (Debranching.state_convert (dom ?\<Pi>\<^sub>B) \<Sigma>\<^sub>B'))" by blast
     with SA' B DL assembly_to_machine_correct obtain \<Sigma>\<^sub>M' where SM': 
-      "\<Sigma>\<^sub>M' \<in> AssemblyToMachine.state_convert (linearize ?\<Pi>\<^sub>A) (Linearization.state_convert \<Sigma>\<^sub>A') \<and> 
-        iterate (eval_machine ?\<Pi>\<^sub>M) \<Sigma>\<^sub>M \<Sigma>\<^sub>M'" by blast
-    with SA' SB' have "\<Sigma>\<^sub>M' \<in> { \<Sigma>\<^sub>M' | \<Sigma>\<^sub>B' \<Sigma>\<^sub>A' \<Sigma>\<^sub>M'. 
+      "\<Sigma>\<^sub>M' \<in> AssemblyToMachine.state_convert (linearize ?\<Pi>\<^sub>A) 
+        (Linearization.state_convert (Debranching.state_convert (dom ?\<Pi>\<^sub>B) \<Sigma>\<^sub>B')) \<and> 
+          iterate (eval_machine ?\<Pi>\<^sub>M) \<Sigma>\<^sub>M \<Sigma>\<^sub>M'" by blast
+    with SA' SB' have "\<Sigma>\<^sub>M' \<in> { \<Sigma>\<^sub>M' | \<Sigma>\<^sub>B' \<Sigma>\<^sub>M'. 
       \<Sigma>\<^sub>B' \<in> StackToAssembly.state_convert \<Sigma>\<^sub>S' \<and> 
-        \<Sigma>\<^sub>A' \<in> Debranching.state_convert (dom ?\<Pi>\<^sub>B) \<Sigma>\<^sub>B' \<and>
-          \<Sigma>\<^sub>M' \<in> AssemblyToMachine.state_convert (linearize ?\<Pi>\<^sub>A) (Linearization.state_convert \<Sigma>\<^sub>A') }" 
+        \<Sigma>\<^sub>M' \<in> AssemblyToMachine.state_convert (linearize ?\<Pi>\<^sub>A) 
+          (Linearization.state_convert (Debranching.state_convert (dom ?\<Pi>\<^sub>B) \<Sigma>\<^sub>B')) }" 
       by blast
     with SM' have "\<Sigma>\<^sub>M' \<in> state_convert \<Pi> \<Sigma>\<^sub>S' \<and> iterate (eval_machine (program_convert \<Pi>)) \<Sigma>\<^sub>M \<Sigma>\<^sub>M'"
       by (simp add: state_convert_def program_convert_def)
